kinda done

proofs/Barrett/UsingMvcgen.lean
@@ -39,43 +39,63 @@ theorem HShiftRight.hShiftRightI64I64.spec (a : I64) (b : I64) (hb : b.bv < 64) 
 theorem Result.ok.spec (a : I64) : ⦃ ⌜ True ⌝ ⦄ Result.ok a ⦃⇓ r => ⌜ r.bv = a.bv ⌝ ⦄ := by
   mvcgen
 
-theorem IScalar.bv_I64ofInt : (I64.ofInt n hn).bv = BitVec.ofInt 64 n := by sorry
-theorem IScalar.bv_I32ofInt : (I32.ofInt n hn).bv = BitVec.ofInt 32 n := by sorry
+
+@[spec]
+theorem Result.ok32.spec (a : I32) : ⦃ ⌜ True ⌝ ⦄ Result.ok a ⦃⇓ r => ⌜ r.bv = a.bv ⌝ ⦄ := by
+  mvcgen
+
+theorem IScalar.bv_I64ofInt : (I64.ofInt n hn).bv = BitVec.ofInt 64 n := by rfl
+theorem IScalar.bv_I32ofInt : (I32.ofInt n hn).bv = BitVec.ofInt 32 n := by rfl
 
 theorem IScalar.cast_val64 :
   @Int.cast (BitVec 64) BitVec.instIntCast
-  (@IScalar.val IScalarTy.I64 n : ℤ) = n.bv := by sorry
+  (@IScalar.val IScalarTy.I64 n : ℤ) = n.bv := by rw [I64.Nat_cast_BitVec_val]
 
 
 theorem IScalar.cast_val32 :
   @Int.cast (BitVec 32) BitVec.instIntCast
-  (@IScalar.val IScalarTy.I32 n : ℤ) = n.bv := by sorry
+  (@IScalar.val IScalarTy.I32 n : ℤ) = n.bv := by rw [I32.Nat_cast_BitVec_val]
 
-theorem IScalar.bv_mkI64 : (@IScalar.mk IScalarTy.I64 x).bv = x := sorry
-theorem IScalar.bv_mkI32 : (@IScalar.mk IScalarTy.I32 x).bv = x := sorry
+theorem IScalar.bv_mkI64 : (@IScalar.mk IScalarTy.I64 x).bv = x := rfl
+theorem IScalar.bv_mkI32 : (@IScalar.mk IScalarTy.I32 x).bv = x := rfl
 
-@[bv_normalize]
-theorem xx :
-   IScalarTy.I64.numBits = 64 := sorry
+-- @[bv_normalize]
+-- theorem xx :
+--    IScalarTy.I64.numBits = 64 := rfl
+
+#check IScalar.cast
+
 
 def wrapper (a : I64) : BitVec 64 := a.bv
 theorem xxxx (a : I64) : a.bv = wrapper a := by rfl
+
+
+def wrapper32 (a : I32) : BitVec 32 := a.bv
+theorem xxxx32 (a : I32) : a.bv = wrapper32 a := by rfl
+
+
 
 open barrett
 
 set_option trace.Meta.Tactic.bv true
 
 theorem barrett_reduce.spec (value : I32)
-    (h1 : (core.convert.num.FromI64I32.from value).bv >= - BARRETT_R.bv)
-    (h2 : (core.convert.num.FromI64I32.from value).bv <= BARRETT_R.bv) :
-    ⦃ ⌜ True ⌝ ⦄ barrett_reduce value ⦃⇓ r => ⌜ True ⌝ ⦄ := by
+    (h1 : BitVec.sle (- BARRETT_R.bv) (core.convert.num.FromI64I32.from value).bv)
+    (h2 : BitVec.sle (core.convert.num.FromI64I32.from value).bv BARRETT_R.bv) :
+    ⦃ ⌜ True ⌝ ⦄
+    barrett_reduce value
+    ⦃⇓ r => ⌜
+    BitVec.slt (- FIELD_MODULUS.bv) r.bv ∧ BitVec.slt r.bv FIELD_MODULUS.bv
+    ∧ r.bv.smod FIELD_MODULUS.bv = value.bv.smod FIELD_MODULUS.bv
+    ⌝ ⦄ := by
   unfold barrett_reduce BARRETT_MULTIPLIER BARRETT_SHIFT FIELD_MODULUS BARRETT_R at *
   mvcgen
   all_goals try simp only [
     IScalar.bv_I64ofInt, IScalar.bv_mkI64, IScalar.bv_I32ofInt, IScalar.bv_mkI32,
     IScalar.cast_val64, IScalar.cast_val32, IScalarTy.numBits,
-    core.convert.num.FromI64I32.from] at *
-  all_goals try simp only [xxxx] at *
+    core.convert.num.FromI64I32.from, IScalar.cast] at *
+  all_goals try simp only [xxxx, xxxx32] at *
   · bv_decide
   · bv_decide
   · bv_decide
+  · bv_decide (timeout := 1200)
